\documentclass{article}

\usepackage[margin=0.5in]{geometry}
\usepackage{amsfonts,xcolor}
\usepackage{amsmath, amsthm} % The package amsmath will make it so that the \text{ words here } things work in the sets $S$ and $T$.

\newcommand\Z{\mathbb{Z}}
\newcommand\Q{\mathbb{Q}}
\newcommand\R{\mathbb{R}}
\newcommand\C{\mathbb{C}}

\begin{document}

\begin{enumerate}

\item Let $f : M \to N$ and $g: N \to L$ both be surjective functions. Prove that $g  \circ f$ is surjective. (First, look carefully at what the domain and codomain of $g \circ f$ are. Of course, be sure to follow the definition of surjective EXACTLY, and do not ignore quantifiers. Determine which ``for all'' is being used and which ``for all'' is being proved, and which ``there exists'' is being used and which ``there exists'' is being proved.)

\begin{proof}
    To prove that $g \circ f$ is surjective, we must show that for all $\ell \in L$, there exists $m \in M$ such that $(g \circ f)(m) = \ell$.

    Let $\ell \in L$ be arbitrary.
    Since $g$ is surjective, there exists $n \in N$ such that $g(n) = \ell$.
    Since $f$ is surjective, there exists $m \in M$ such that $f(m) = n$.

    Therefore, $(g \circ f)(m) = g(f(m)) = g(n) = \ell$.

    Thus, for all $\ell \in L$, there exists $m \in M$ such that $(g \circ f)(m) = \ell$, proving that $g \circ f$ is surjective.
\end{proof}

\newpage

\item Let $f : M \to N$ and $g: N \to L$ both be injective functions. Prove that $g  \circ f$ is injective. (The same types of hints as the previous question, and in fact, at this level of math, the following advice always applies: since the question mentions the word injective, go review the definition first and do NOT ignore quantifiers. Determine which ``for all'' is being used and which ``for all'' is being proved.)

\begin{proof}
    To prove that $g \circ f$ is injective, we must show that for all $m_1, m_2 \in M$, if $(g \circ f)(m_1) = (g \circ f)(m_2)$, then $m_1 = m_2$.

    Let $m_1, m_2 \in M$ be arbitrary and assume $(g \circ f)(m_1) = (g \circ f)(m_2)$.
    Then $g(f(m_1)) = g(f(m_2))$.
    Since $g$ is injective, this implies $f(m_1) = f(m_2)$.
    Since $f$ is injective, this implies $m_1 = m_2$.

    Thus, for all $m_1, m_2 \in M$, if $(g \circ f)(m_1) = (g \circ f)(m_2)$, then $m_1 = m_2$, proving that $g \circ f$ is injective.
\end{proof}

\newpage

\item Let $f : M \to N$. Prove: if $A$ and $B$ are subsets of $N$ such that $A \subseteq B$, then $f^{-1}(A) \subseteq f^{-1}(B)$.

\begin{proof}
    To prove that $f^{-1}(A) \subseteq f^{-1}(B)$, we must show that for all $x \in f^{-1}(A)$, $x \in f^{-1}(B)$.

    Let $x \in f^{-1}(A)$ be arbitrary.
    By definition of preimage, this means $f(x) \in A$.
    Since $A \subseteq B$, this implies $f(x) \in B$.
    By definition of preimage, this means $x \in f^{-1}(B)$.

    Thus, for all $x \in f^{-1}(A)$, $x \in f^{-1}(B)$, proving that $f^{-1}(A) \subseteq f^{-1}(B)$.
\end{proof}

\newpage

\item Prove that $[2,6]$ and $[11,20]$ are equicardinal. For clarifcation, both sets/intervals mentioned are subsets of $\mathbb{R}$.

\newpage

\begin{proof}
    To prove that [2,6] and [11,20] are equicardinal, we need to find a bijective function between them.

    Let f: [2,6] → [11,20] be defined by f(x) = 3x + 5.

    First, let's prove f is injective:
    Let x₁, x₂ ∈ [2,6] and assume f(x₁) = f(x₂).
    Then 3x₁ + 5 = 3x₂ + 5
    Therefore x₁ = x₂, proving f is injective.

    Now, let's prove f is surjective:
    Let y ∈ [11,20] be arbitrary.
    Let x = (y-5)/3.
    Then f(x) = y, and we need to verify x ∈ [2,6].
    When y = 11, x = 2
    When y = 20, x = 5
    Since f is linear and continuous, x ∈ [2,6].
    Therefore f(x) = y for some x ∈ [2,6].

    Since f is both injective and surjective, it is bijective.
    Therefore [2,6] and [11,20] are equicardinal.
\end{proof}

\item Prove: if $A$ is countably infinite and $B$ is countably infinite and $C$ is countably infinite and $A \cap B = \emptyset$ and $A \cap C= \emptyset$ and $B \cap C = \emptyset$, prove $A \cup B \cup C$ is countably infinite. (Hint: it will be helpful to look at a past HW key where a formula for a sequence was given.)

\end{enumerate}
    \begin{proof}
        Since A is countably infinite, there exists a bijection f: ℕ → A.
        Since B is countably infinite, there exists a bijection g: ℕ → B.
        Since C is countably infinite, there exists a bijection h: ℕ → C.

        Define φ: ℕ → A ∪ B ∪ C by:
        φ(n) = \begin{cases}
            f(k) & \text{if } n = 3k-2 \text{ for some } k \in ℕ \\
            g(k) & \text{if } n = 3k-1 \text{ for some } k \in ℕ \\
            h(k) & \text{if } n = 3k \text{ for some } k \in ℕ
        \end{cases}

        To prove φ is injective:
        Let n₁, n₂ ∈ ℕ with φ(n₁) = φ(n₂).
        If n₁, n₂ came from different cases, they would map to different sets (A, B, or C), which are disjoint.
        If from the same case, f, g, h being injective implies n₁ = n₂.
        Thus φ is injective.

        To prove φ is surjective:
        Let x ∈ A ∪ B ∪ C.
        If x ∈ A, then x = f(k) for some k, so x = φ(3k-2).
        If x ∈ B, then x = g(k) for some k, so x = φ(3k-1).
        If x ∈ C, then x = h(k) for some k, so x = φ(3k).
        Thus φ is surjective.

        Therefore A ∪ B ∪ C is countably infinite.
    \end{proof}
\end{document}
